lib_list/Selectors.LList.fsti
@@ -40,34 +40,34 @@ val is_null_t (#a:Type) (ptr:t a) : (b:bool{b <==> ptr == null_t})
 val llist_sl (#a:Type0) (p: a -> vprop) (r: t a): slprop u#1
 /// Selector of a list. Returns an F* list of elements of type [a]
 
-val llist_sel (#a:Type0) (p : a -> vprop) (r:t a) : selector (list a) (llist_sl p r)
+val llist_sel (#a:Type0) (p: a -> vprop) (r:t a) : selector (list a) (llist_sl p r)
 
 /// Combining the two above into a linked list vprop
 [@@__steel_reduce__]
-let llist' #a (p : a -> vprop) r : vprop' =
+let llist' #a (p: a -> vprop) r : vprop' =
   {hp = llist_sl p r;
    t = list a;
    sel = llist_sel p r}
 unfold
-let llist (#a:Type0) (p : a -> vprop) (r:t a) = VUnit (llist' p r)
+let llist (#a:Type0) (p: a -> vprop) (r:t a) = VUnit (llist' p r)
 
 /// A wrapper to access a list selector more easily.
 /// Ensuring that the corresponding llist vprop is in the context is done by
 /// calling a variant of the framing tactic, as defined in Steel.Effect.Common
 [@@ __steel_reduce__]
-let v_llist (#a:Type0) (#p2:vprop) (p : a -> vprop) (r:t a)
+let v_llist (#a:Type0) (#p2:vprop) (p: a -> vprop) (r:t a)
   (h:rmem p2{FStar.Tactics.with_tactic selector_tactic (can_be_split p2 (llist p r) /\ True)}) : GTot (list a)
   = h (llist p r)
 
 (** Stateful lemmas to fold and unfold the llist predicate **)
 
-val intro_llist_nil (#opened:inames) (#a:Type0) (p : a -> vprop)
+val intro_llist_nil (#opened:inames) (#a:Type0) (p: a -> vprop)
   : SteelGhost unit opened
     emp (fun _ -> llist p (null_t #a))
     (requires fun _ -> True)
     (ensures fun _ _ h1 -> v_llist #a p null_t h1 == [])
 
-val elim_llist_nil (#opened:inames) (#a:Type0) (p : a -> vprop) (ptr:t a)
+val elim_llist_nil (#opened:inames) (#a:Type0) (p: a -> vprop) (ptr:t a)
   : SteelGhost unit opened
   (llist p ptr) (fun _ -> llist p ptr)
   (requires fun _ -> ptr == null_t)
@@ -75,7 +75,7 @@ val elim_llist_nil (#opened:inames) (#a:Type0) (p : a -> vprop) (ptr:t a)
     v_llist p ptr h0 == v_llist p ptr h1 /\
     v_llist p ptr h1 == [])
 
-val cons_is_not_null (#opened:inames) (#a:Type0) (p : a -> vprop) (ptr:t a)
+val cons_is_not_null (#opened:inames) (#a:Type0) (p: a -> vprop) (ptr:t a)
   : SteelGhost unit opened
   (llist p ptr) (fun _ -> llist p ptr)
   (requires fun h -> Cons? (v_llist p ptr h))
@@ -86,6 +86,7 @@ val cons_is_not_null (#opened:inames) (#a:Type0) (p : a -> vprop) (ptr:t a)
 // val null_is_nil
 // val nil_is_null
 // val not_null_is_cons
+
 
 val pack_list (#opened:inames) (#a:Type0)
   (p: a -> vprop)
@@ -117,37 +118,36 @@ val unpack_list (#a:Type0)
       (get_data (sel ptr h1)) :: (v_llist p (get_next n) h1) /\
      sel ptr h1 == n)
 
-(*)
 (** A variant of lists with an additional indirection pointer to enable in-place operations **)
 
-val ind_llist_sl (#a:Type0) (r:ref (t a)) : slprop u#1
-val ind_llist_sel (#a:Type0) (r:ref (t a)) : selector (list a) (ind_llist_sl r)
+val ind_llist_sl (#a:Type0) (p: a -> vprop) (r:ref (t a)) : slprop u#1
+val ind_llist_sel (#a:Type0) (p: a -> vprop) (r:ref (t a)) : selector (list a) (ind_llist_sl p r)
 
 [@@__steel_reduce__]
-let ind_llist' (#a:Type0) (r:ref (t a)) : vprop' =
-  { hp = ind_llist_sl r;
+let ind_llist' (#a:Type0) (p: a -> vprop) (r:ref (t a)) : vprop' =
+  { hp = ind_llist_sl p r;
     t = list a;
-    sel = ind_llist_sel r}
+    sel = ind_llist_sel p r}
 unfold
-let ind_llist (#a:Type0) (r:ref (t a)) = VUnit (ind_llist' r)
+let ind_llist (#a:Type0) (p: a -> vprop) (r:ref (t a)) = VUnit (ind_llist' p r)
 
 [@@ __steel_reduce__]
-let v_ind_llist (#a:Type0) (#p:vprop) (r:ref (t a))
-  (h:rmem p{FStar.Tactics.with_tactic selector_tactic (can_be_split p (ind_llist r) /\ True)}) : GTot (list a)
-  = h (ind_llist r)
+let v_ind_llist (#a:Type0) (#p2:vprop) (p: a -> vprop) (r:ref (t a))
+  (h:rmem p2{FStar.Tactics.with_tactic selector_tactic (can_be_split p2 (ind_llist p r) /\ True)}) : GTot (list a)
+  = h (ind_llist p r)
 
-val unpack_ind (#a:Type0) (r:ref (t a))
+val unpack_ind (#a:Type0) (p: a -> vprop) (r:ref (t a))
   : Steel (t a)
-             (ind_llist r)
-             (fun p -> vptr r `star` llist p)
-             (requires fun _ -> True)
-             (ensures fun h0 p h1 ->
-               sel r h1 == p /\
-               v_llist p h1 == v_ind_llist r h0)
+  (ind_llist p r)
+  (fun r2 -> vptr r `star` llist p r2)
+  (requires fun _ -> True)
+  (ensures fun h0 r2 h1 ->
+    sel r h1 == r2 /\
+    v_llist p r2 h1 == v_ind_llist p r h0)
 
-val pack_ind (#a:Type0) (r:ref (t a)) (p:t a)
-  : Steel unit
-             (vptr r `star` llist p)
-             (fun _ -> ind_llist r)
-             (requires fun h -> sel r h == p)
-             (ensures fun h0 _ h1 -> v_llist p h0 == v_ind_llist r h1)
+val pack_ind (#opened:inames) (#a:Type0) (p: a -> vprop) (r:ref (t a)) (r2:t a)
+  : SteelGhost unit opened
+  (vptr r `star` llist p r2)
+  (fun _ -> ind_llist p r)
+  (requires fun h -> sel r h == r2)
+  (ensures fun h0 _ h1 -> v_llist p r2 h0 == v_ind_llist p r h1)
